automation update

Algebraic_Group_Model.thy
@@ -2,9 +2,7 @@ theory Algebraic_Group_Model
   imports CryptHOL.CryptHOL Restrictive_Comp
   keywords
   "lift_to_algebraicT" :: thy_decl
-and  "AGMLifting" :: thy_decl
-and "lift_to_algebraic" :: thy_decl
-and "lift_to_AGM" :: thy_decl
+and "agm_interpretation" :: thy_decl
 begin
 
 text \<open>This theory extends CryptHOL for the Algebraic Group Model according to 
@@ -16,67 +14,23 @@ cannot ensure that the adversary algorithm itself is algebraic. Instead we enfor
 rules on the outputs of the adversary, counting rule breaking as losing the game. Hence, every 
 adversary with non-negligible advantage has to be an algebraic algorithm.
 
-We formalize the algebraic rules in the functions 'constrain' and 'constrain_list', which enforce 
-the algebraic rules for one/resp. a list of output pair/s.
+We formalize this relaxed notion of an algebraic algorithm as a sub case of Restrictive_Comp, i.e. 
+we define the AGM in terms of a RCM.
 
-We provide ML functions to enforce the rules of an algebraic algorithm on specific and
-arbitrary algorithms thereby practically lifting adversaries from the standard model to the AGM. 
-Finally, we provide the ML function 'lift_to_agm' that takes any game in the standard model and 
-automatically derives it's definition in the AGM.
-\<close>
+We provide group specific records groupS and groupC for Select and constrain. Furthermore,  
+we define some automation and sanity check functions in Isabelle/ML\<close>
 
-(* General methodology: 
-select - filters the relevant group elements from the inputs in a generic way so ML can use the 
-things
-constrain::'b list \<Rightarrow> 'c \<Rightarrow> bool - enforces constrains on a single element 
-
-Built relevant lemmas about lists and prods around this
-Built one manual AGM encapsulating do {assert and return} block in Isabelle/HOL
-The ML task is to assemble all these from a big game in one call *)
-(* TODO implement ML part to infer the part within the control arrows for select and constrain 
-e.g. prodC (listC gC) gC from ([g,g^2,g^3], g)*)
-
-locale algebraic_algorithm = cyclic_group 
+context cyclic_group
 begin
 
 text \<open>group elements are the single important type we want to select.\<close>
-definition groupS :: "('a,'a) restrictive_comp_sel"
+definition groupS :: "('a,'a) Select"
   where "groupS \<equiv> \<lparr>select = (\<lambda>x. [x])\<rparr>"
-
-text \<open>atomic types don't harbour group elements\<close>
-
-definition boolS :: "(bool,'a) restrictive_comp_sel"
-  where "boolS \<equiv> \<lparr>select = (\<lambda>x. [])\<rparr>"
-
-definition unitS :: "(unit,'a) restrictive_comp_sel"
-  where "unitS \<equiv> \<lparr>select = (\<lambda>x. [])\<rparr>"
-
-definition natS :: "(nat,'a) restrictive_comp_sel"
-  where "natS \<equiv> \<lparr>select = (\<lambda>x. [])\<rparr>"
-
-definition intS :: "(int,'a) restrictive_comp_sel"
-  where "intS \<equiv> \<lparr>select = (\<lambda>x. [])\<rparr>"
-
-definition ratS :: "(rat,'a) restrictive_comp_sel"
-  where "ratS \<equiv> \<lparr>select = (\<lambda>x. [])\<rparr>"
-
-definition realS :: "(real,'a) restrictive_comp_sel"
-  where "realS \<equiv> \<lparr>select = (\<lambda>x. [])\<rparr>"
-
-definition complexS :: "(complex,'a) restrictive_comp_sel"
-  where "complexS \<equiv> \<lparr>select = (\<lambda>x. [])\<rparr>"
-
-definition charS :: "(char,'a) restrictive_comp_sel"
-  where "charS \<equiv> \<lparr>select = (\<lambda>x. [])\<rparr>"
-
-definition stringS :: "(string,'a) restrictive_comp_sel"
-  where "stringS \<equiv> \<lparr>select = (\<lambda>x. [])\<rparr>"
 
 text \<open>The above definitions can be composed with the existing data structure extensions from 
 Restrictive_Comp and should cover a wide range of possible inputs. In case some case is missing, 
 the Restrictive_Comp records can be extended to more data structures (see Restrictive_Comp for 
 examples) and this locale can be extended for more atomic type definitions.\<close>
-
 
 text \<open>check the rules of an algebraic algorithm i.e. given the elements g, a group element, 
 and the vector vec=[c_0,...c_n] from the algorithm ensure that g=s_0 [^] c_0 \<otimes> ... \<otimes>
@@ -86,42 +40,10 @@ definition constrain_grp :: "'a list \<Rightarrow> ('a \<times> int list) \<Righ
   where "constrain_grp seen_vec res \<equiv> 
     let (g,c_vec) = res in
     (length seen_vec = length c_vec 
-    \<and> g = fold (\<lambda> i acc. acc \<otimes> seen_vec!i [^] (c_vec!i)) [0..<length seen_vec] \<one>)"
+    \<and> g = fold (\<lambda> i acc. acc \<otimes>\<^bsub>G\<^esub> seen_vec!i [^]\<^bsub>G\<^esub> (c_vec!i)) [0..<length seen_vec] \<one>\<^bsub>G\<^esub>)"
 
-definition groupC :: "(('a \<times> int list), 'a) restrictive_comp_con"
+definition groupC :: "('a, ('a \<times> int list)) Constrain"
   where "groupC \<equiv> \<lparr>constrain = (\<lambda>ip op. constrain_grp ip op)\<rparr>"
-
-text \<open>We don't need to constrain atomic types\<close>
-
-definition constrain_atomic :: "'a list \<Rightarrow> 'b \<Rightarrow> bool" 
-  where "constrain_atomic seen_vec res \<equiv> True"
-
-definition boolC :: "(bool, 'a) restrictive_comp_con"
-  where "boolC \<equiv> \<lparr>constrain = (\<lambda>ip op. True)\<rparr>"
-
-definition unitC :: "(unit,'a) restrictive_comp_con"
-  where "unitC \<equiv> \<lparr>constrain = (\<lambda>ip op. True)\<rparr>"
-
-definition natC :: "(nat, 'a) restrictive_comp_con"
-  where "natC \<equiv> \<lparr>constrain = (\<lambda>ip op. True)\<rparr>"
-
-definition intC :: "(int, 'a) restrictive_comp_con"
-  where "intC \<equiv> \<lparr>constrain = (\<lambda>ip op. True)\<rparr>"
-
-definition ratC :: "(rat, 'a) restrictive_comp_con"
-  where "ratC \<equiv> \<lparr>constrain = (\<lambda>ip op. True)\<rparr>"
-
-definition realC :: "(real, 'a) restrictive_comp_con"
-  where "realC \<equiv> \<lparr>constrain = (\<lambda>ip op. True)\<rparr>"
-
-definition complexC :: "(complex, 'a) restrictive_comp_con"
-  where "complexC \<equiv> \<lparr>constrain = (\<lambda>ip op. True)\<rparr>"
-
-definition charC :: "(char, 'a) restrictive_comp_con"
-  where "charC \<equiv> \<lparr>constrain = (\<lambda>ip op. True)\<rparr>"
-
-definition stringC :: "(string, 'a) restrictive_comp_con"
-  where "stringC \<equiv> \<lparr>constrain = (\<lambda>ip op. True)\<rparr>"
 
 text \<open>group values that follow the rules of an algebraic algorithm are actually in the group\<close>
 lemma constrain_grp_is_in_carrier:
@@ -180,10 +102,18 @@ proof -
   finally show "g \<in> carrier G" by blast
 qed
 
-end 
+end
 
-locale algebraic_algorithm_examples = algebraic_algorithm
-begin 
+locale Algebraic_Algorithm = G : cyclic_group G 
+  for G :: "('a, 'b) cyclic_group_scheme" (structure)
+  + 
+  fixes sel :: "('x,'a) Select"
+  and con :: "('a,'y) Constrain"
+
+sublocale Algebraic_Algorithm \<subseteq> Restrictive_Comp sel con .
+
+locale algebraic_algorithm_examples = cyclic_group
+begin
 
 text \<open>To obtain an algebraic algorithm one needs to simply instantiate the restrictive_comp locale 
 with the record composition that one needs and apply the non-algebraic algorithm to the obtained 
@@ -195,13 +125,14 @@ text \<open>For simplicity let the adversary be id\<close>
 definition \<A>_id :: "'a \<Rightarrow> ('a \<times> int list) spmf" 
   where "\<A>_id = (\<lambda>x. return_spmf (x, [1::int]))"
 
-interpretation id: restrictive_comp groupS groupC .
+interpretation Algebraic_Algorithm G "groupS" "groupC" 
+  by (unfold_locales) 
 
 lemma 
   assumes "g \<in> carrier G"
-  shows "id.restrict \<A>_id g
+  shows "restrict \<A>_id g
     = \<A>_id g"
-  unfolding \<A>_id_def restrictive_comp.restrict_def
+  unfolding \<A>_id_def Restrictive_Comp.restrict_def 
   unfolding groupS_def groupC_def constrain_grp_def
   by (simp add: assms)
   
@@ -210,727 +141,232 @@ text \<open>Now the same for a list of input elements and and output elements\<c
 definition \<A>_list_fst :: "'a list \<Rightarrow> ('a \<times> int list) list spmf" 
   where "\<A>_list_fst = (\<lambda>x. return_spmf (map (\<lambda>_. (x!0, [1::int,0,0])) x))"
 
-interpretation list_id: restrictive_comp "(listS groupS)" "listC groupC" .
+interpretation list_id: Restrictive_Comp "(listS groupS)" "listC groupC" .
 
 lemma 
   assumes "g1 \<in> carrier G \<and> g2 \<in> carrier G \<and> g3 \<in> carrier G"
   shows "list_id.restrict \<A>_list_fst [g1,g2,g3]
     = \<A>_list_fst [g1,g2,g3]"
-  unfolding \<A>_list_fst_def restrictive_comp.restrict_def
-  unfolding groupS_def groupC_def listS_def listC_def constrain_grp_def
+  unfolding \<A>_list_fst_def Restrictive_Comp.restrict_def
+  unfolding listS_def groupS_def listC_def groupC_def 
+    unfolding constrain_grp_def
   by (simp add: assms)
 
-end
+text \<open>We define some useful ML functions for the AGM.
 
+wellformed is a sanity check that checks, given a group G and a function type, that the function 
+type returns a creation vector (int list) paired with every group value in the output.  
 
-
-
-
-
-
-
-
-
-
-
-
-
-
-
-context cyclic_group
-begin
-
-text \<open>check the rules of an algebraic algorithm i.e. given the elements g, a group element, 
-and the vector vec=[c_0,...c_n] from the algorithm ensure that g=s_0 [^] c_0 \<otimes> ... \<otimes>
-s_0 [^] c_0, where [s_0,...,s_n]=seen are the group values the algorithm was supplied with.
-\<close>
-fun constrain :: "'a list \<Rightarrow> 'a \<Rightarrow> (int list) \<Rightarrow> bool"
-  where "constrain seen_vec g c_vec = (length seen_vec = length c_vec 
-    \<and> g = fold (\<lambda> i acc. acc \<otimes> seen_vec!i [^] (c_vec!i)) [0..<length seen_vec] \<one>)"
-
-text \<open>Given a list of (seen) group elements and vectors from an algebraic algorithm, 
-constrain all of them to the rules of algebraic algorithms\<close>
-fun constrain_list :: "'a list \<Rightarrow> ('a \<times> int list) list \<Rightarrow> bool"
-  where "constrain_list seen xs = list_all (\<lambda>(g, c_vec). constrain seen g c_vec) xs"
-
-text \<open>group values that follow the rules of an algebraic algorithm are actually in the group\<close>
-lemma constrain_is_in_carrier:
-  assumes "\<forall>g \<in> set seen_vec. g \<in> carrier G"
-  and "constrain seen_vec g c_vec"
-shows "g \<in> carrier G"
-proof -
-  have "g = fold (\<lambda> i acc. acc \<otimes> seen_vec!i [^] (c_vec!i)) [0..<length seen_vec] \<one>"
-    using assms(2) by simp
-  also have "length seen_vec = length c_vec"
-    using assms(2) by fastforce
-  then have "fold (\<lambda> i acc. acc \<otimes> seen_vec!i [^] (c_vec!i)) [0..<length seen_vec] \<one> \<in> carrier G" 
-    using assms(1)
-  proof (induct seen_vec c_vec rule: rev_induct2)
-    case (4 x xs y ys)
-    then have fold_xs_carrier: "fold (\<lambda>i acc. acc \<otimes> xs ! i [^] ys ! i) [0..<length xs] \<one> \<in> carrier G"
-      by fastforce
-    moreover have "x [^] y \<in> carrier G"
-      by (simp add: 4(3))
-    moreover have "fold (\<lambda>i acc. acc \<otimes> (xs @ [x]) ! i [^] (ys @ [y]) ! i) [0..<length (xs @ [x])] \<one> 
-      =  (fold (\<lambda>i acc. acc \<otimes> xs ! i [^] ys ! i) [0..<length xs] \<one>) \<otimes> x [^] y"
-    proof -
-      let ?fyys = "\<lambda>xs::'a list. (\<lambda>i acc. acc \<otimes> xs ! i [^] (ys @ [y]) ! i)"
-      have "fold (\<lambda>i acc. acc \<otimes> (xs @ [x]) ! i [^] (ys @ [y]) ! i) [0..<length (xs @ [x])] \<one> 
-        = fold (?fyys (xs@[x])) [0..<length (xs @ [x])] \<one>" by blast
-      moreover have "\<dots> = (fold (?fyys (xs@[x])) [length (xs @ [x]) - 1] \<circ> fold (?fyys (xs@[x])) [0..<length (xs)]) \<one>"
-        by auto
-      moreover have "\<dots> = ((\<lambda>acc. acc \<otimes> x [^] y)  \<circ> fold (?fyys (xs@[x])) [0..<length (xs)]) \<one>"
-        by (smt (verit, del_insts) "4"(2) One_nat_def add_Suc_right append.right_neutral diff_Suc_Suc diff_zero fold.simps(1) fold_Cons id_comp
-            length_append list.size(3,4) nth_append_length o_apply)
-      moreover have "\<dots> = (fold (?fyys (xs@[x])) [0..<length (xs)] \<one>) \<otimes> x [^] y"
-        by force
-      moreover have "\<dots> = (fold (\<lambda>i acc. acc \<otimes> xs ! i [^] ys ! i) [0..<length (xs)] \<one>) \<otimes> x [^] y"
-      proof - 
-        have "fold (?fyys (xs@[x])) [0..<length (xs)] \<one>
-          = fold (\<lambda>i acc. acc \<otimes> xs ! i [^] ys ! i) [0..<length xs] \<one>"
-        proof(rule fold_cong)
-          fix xa
-          assume "xa \<in> set [0..<length xs]"
-          then have xs_le_xs: "xa < length xs" 
-            by force
-          then have "(xs @ [x]) ! xa = xs ! xa"
-            using nth_append_left by blast
-          moreover have "(ys @ [y]) ! xa = ys ! xa"
-            using 4(2) nth_append_left xs_le_xs by auto
-          ultimately show "(\<lambda>acc. acc \<otimes> (xs @ [x]) ! xa [^] (ys @ [y]) ! xa) = (\<lambda>acc. acc \<otimes> xs ! xa [^] ys ! xa)"
-            by presburger
-        qed force+
-        then show ?thesis by presburger
-      qed
-      ultimately show ?thesis by argo
-    qed
-    ultimately show ?case
-      by auto
-  qed force+
-  finally show "g \<in> carrier G" by blast
-qed
-
-subsection \<open>Algebraic Algorithm\<close>
-
-text \<open>ML functions that enforce algebraic rules on different objects.
-
-lift_to_algebraicT operates on the type level, lifiting standard model function types into their 
+lift_to_algebraicT operates on the type level, lifting standard model function types into their 
 corresponding type as an algebraic algorithm. I.e. extend the outputs that are group elements 
 with a vector.
 
-enforce_alg enforces the algebraic rules on a specific probabilistic algorithm. 
-Effectively turning any probabilistic algorithm into an algebraic algorithm.
-Probabilistic in this case means the algorithm has to return a spmf value. If the algorithm breaks the 
-algebraic rules, enforce_alg returns None.
-
-build_alg_fun takes a certain type T and builds a function that takes any probabilistic 
-(probabilistic defined as before) algorithm \<A> of that type and returns the algebraic algorithm 
-obtained by computing enforce_alg for \<A>.
-
-lift_to_agm takes a game in standard model and turns it into a game in the algebraic group model.
-\<close>
-
-ML \<open>
-signature ALGEBRAIC_ALGORITHM =
-sig 
-
-
-val lift_to_algebraicT : typ -> typ -> typ -> typ
-
-val extract_type_params : typ -> string list
-
-val enforce_alg: Name.context -> term -> term -> term
-
-val build_alg_fun : Name.context -> term -> typ -> term
-
-val lift_to_agm : theory -> Proof.context -> term -> term -> term list -> term list -> term
-
-end;
-
-structure Algebraic_Algorithm : ALGEBRAIC_ALGORITHM = 
-struct
-
-(* Functions relevant for lifting a standard model adversary type to an algebraic adversary type 
-i.e lift_to_algebraicT *)
-
-fun rcodomain_transf f (Type ("fun", [T, U])) = (Type ("fun", [T, rcodomain_transf f U]))
-  | rcodomain_transf f T = f T;
-
-fun adjoin t vec = fn T => if T = t then Type ("Product_Type.prod", [T, vec]) else T
-
-fun lift_to_algebraicT grpT vec = (rcodomain_transf o Term.map_atyps) (adjoin grpT vec)
-
-(* Functions relevant for enforcing algebraic rules on a concrete (suitable typed) algorithm. I.e. 
-lift_to_algebraic *)
-
-fun strip_spmfT T = T 
-    |> Term.dest_Type_args 
-    |> hd 
-    |> Term.dest_Type_args 
-    |> hd 
-
-fun return_spmf t = 
-  let 
-    val T = Term.fastype_of t 
-  in 
-    \<^Const>\<open>return_pmf \<^Type>\<open>option T\<close> for \<^Const>\<open>Some T for t\<close>\<close>
-  end
-
-fun extract_type_params t = Term.add_tfree_namesT t []
-
-fun rapply [] t = t
-  | rapply (x::xs) t = rapply xs (t $ x) 
-
-fun rabs [] t = t 
-  | rabs (x::xs) t = rabs xs (Term.lambda x t)
-
-fun create_names_prod_cases nctxt  (Type ("Product_Type.prod", [T1, T2])) = 
-    let 
-      val (T2_res,nctxt') = create_names_prod_cases nctxt T2
-      val (T1_res, nctxt'') = create_names_prod_cases nctxt' T1
-    in 
-      (T1_res@T2_res, nctxt'')
-    end
-  | create_names_prod_cases nctxt T = 
-    let 
-      val (name,nctxt') = Name.variant "" nctxt
-    in 
-      ([Term.Free (name, T)], nctxt') 
-    end;
-
-fun extract_vec_pair_list T (Term.Free(t1N,t1T)::Term.Free(t2N,t2T)::xs) 
-    = if t1T = T andalso t2T = @{typ "int list"} then
-        let 
-          val intlistT =  @{typ "int list"} 
-          val listT = \<^Type>\<open>Product_Type.prod T intlistT\<close>
-          val res = (extract_vec_pair_list T xs)
-          val t1 = Term.Free(t1N,t1T)
-          val t2 = Term.Free(t2N,t2T)
-         in 
-          \<^Const>\<open>List.Cons listT for \<^Const>\<open>Pair T intlistT for t1 t2\<close> res\<close>
-         end
-      else extract_vec_pair_list T xs
-    | extract_vec_pair_list T (_::xs) = extract_vec_pair_list T xs
-    | extract_vec_pair_list T _ =
-      let 
-        val intlistT =  @{typ "int list"} 
-        val listT = \<^Type>\<open>Product_Type.prod T intlistT\<close>
-      in 
-         \<^Const>\<open>list.Nil listT\<close>
-      end
-
-fun extract_seen_list T (Term.Free(tN,tT)::prams) = 
-  let
-    val pram = Term.Free(tN,tT)
-    val seen = extract_seen_list T prams
-  in
-    if 
-      tT = T
-    then 
-       \<^Const>\<open>List.Cons T for pram seen\<close>
-    else if
-      tT = \<^Type>\<open>list T\<close>
-    then 
-      \<^Const>\<open>append T for pram seen\<close>
-    else 
-      seen
-  end
-  | extract_seen_list T _ = \<^Const>\<open>list.Nil T\<close>
-
-fun get_grpTs grp_desc = 
-  let 
-    fun last_type_arg t = t |> Term.dest_Type_args |> tl |> hd
-    val fst_grpT = Term.fastype_of grp_desc |> Term.dest_Type_args |> hd
-    val snd_grpT = Term.fastype_of grp_desc |> last_type_arg |> last_type_arg |> last_type_arg
-  in 
-    (fst_grpT, snd_grpT)
-  end
-
-fun constrain_pairs nctxt grp_desc resT prams = 
-  let 
-    val (grpT1,grpT2) = get_grpTs grp_desc
-    val xs = resT 
-        |> create_names_prod_cases nctxt 
-        |> fst 
-        |> extract_vec_pair_list grpT1
-    val seen = extract_seen_list grpT1 prams
-  in
-     \<^Const>\<open>cyclic_group.constrain_list grpT1 grpT2 for grp_desc seen xs\<close>
-  end
-
-fun create_assert nctxt grp_desc resT prams = 
-  let 
-    val _ = writeln (@{make_string} resT);
-    val assert_term = constrain_pairs nctxt grp_desc resT prams
-  in 
-    \<^Const>\<open>SPMF.assert_spmf for assert_term\<close>
-  end
-
-fun build_ret_term_rec nctxt (Type ("Product_Type.prod", [T1, T2])) = 
-  let 
-    val (t2,nctxt') = build_ret_term_rec nctxt T2
-    val (t1,nctxt'') = build_ret_term_rec nctxt' T1
-  in 
-    (\<^Const>\<open>Pair T1 T2 for t1 t2\<close>, nctxt'')
-  end 
-  | build_ret_term_rec nctxt T = 
-  let 
-    val (name,nctxt') = Name.variant "" nctxt
-  in 
-    (Term.Free (name, T), nctxt') 
-  end;
-
-fun build_ret_term nctxt T = 
-   build_ret_term_rec nctxt T |> fst |> return_spmf
-
-fun abs_typ_over_term_rec (Type ("Product_Type.prod", [T1, T2])) (t,nctxt) = 
-  let 
-    val restT = t |> Term.fastype_of
-    val (rest,nctxt') = abs_typ_over_term_rec T2 (t,nctxt) |> abs_typ_over_term_rec T1
-  in
-     (\<^Const>\<open>Product_Type.prod.case_prod T1 T2 restT\<close> $ rest, nctxt') (*abs T1 (abs T2)*)
-  end
-  | abs_typ_over_term_rec T (t,nctxt) = 
-  let 
-    val (name,nctxt') = Name.variant "" nctxt
-  in 
-    (Term.absfree (name, T) t, nctxt') 
-  end;
-
-fun abs_typ_over_term nctxt T t = abs_typ_over_term_rec T (t,nctxt) |> fst
-
-fun extract_params nctxt T = 
-  let 
-    val (pramsT, _) = Term.strip_type T;
-    val (pNames,nctxt') = Name.invent' "" (length pramsT) nctxt;
-    val prams = map (fn (n,T) => Term.Free (n, T)) (pNames ~~ pramsT)
-  in 
-    (prams, nctxt') 
-  end
-
-fun supply_prams t prams = rapply prams t
-
-fun build_assert_fun nctxt grp_desc retT prams t = 
-  let 
-    val unitT = @{typ unit}
-    val assert_term = create_assert nctxt grp_desc retT prams
-    val t' = Term.absdummy unitT t
-  in
-   \<^Const>\<open>bind_spmf unitT retT for assert_term t'\<close>
-  end
-
-fun build_body_fun nctxt grp_desc T prams = 
-  build_ret_term nctxt T |> build_assert_fun nctxt grp_desc T prams |> abs_typ_over_term nctxt T
-
-fun enforce_alg nctxt grp_desc t = 
-  let 
-    val (prams,nctxt') = Term.fastype_of t |> extract_params nctxt
-    val spmf = supply_prams t prams
-    val retT = Term.fastype_of spmf |> strip_spmfT
-    val body_term = build_body_fun nctxt' grp_desc retT prams
-    val fun_term = \<^Const>\<open>bind_spmf retT retT for spmf body_term\<close>
-  in 
-    rabs (rev prams) fun_term
-  end
-
-(* function that enforces algebraic rules for an arbitrary (suitably typed) algorithm *)
-
-fun build_alg_fun nctxt grp_desc T = 
-  let
-    (* create params to abstract over*)
-    val (prams,nctxt') = extract_params nctxt T
-    (* instantiate the adversary*)
-    val (advN, _) = Name.variant "\<A>" nctxt'
-    val adv = Term.Free(advN,T)
-    (* create the fun term to enforce the agm for the adversary *)
-    val fun_term = enforce_alg nctxt grp_desc adv
-  in 
-    Term.lambda adv fun_term
-  end
-
-(* functions relevant for turning a standard model game in a game in the AGM i.e. lift_to_agm *)
-
-fun get_def_thm thy def = 
-    let 
-      val def_stripped = Term.head_of def
-      val name = (Term.dest_Const_name def_stripped) ^ "_def_raw"
-      val def_thm = Thm.axiom thy name
-    in
-      def_thm
-    end
-
-fun get_def_thm_rhs thy def = 
-    let 
-      val def_thm = get_def_thm thy def
-      val def_content = Thm.concl_of def_thm
-      val rhs = def_content |> Logic.dest_equals |> snd
-    in
-      rhs
-    end
-
-fun get_def_thm_lhs thy def = 
-    let 
-      val def_thm = get_def_thm thy def
-      val def_content = Thm.concl_of def_thm
-      val lhs = def_content |> Logic.dest_equals |> fst
-    in
-      lhs
-    end
-
-exception MATCH;
-
-(* t1 is the term do be matched on a subterm of t2 *)
-fun match_subterms ctxt t1 t2 = 
-   let
-    fun ex t2 = 
-    Thm.match (Thm.cterm_of ctxt t1,Thm.cterm_of ctxt t2)
-    handle Pattern.MATCH => 
-      (case t2 of
-        t $ u => (ex t handle Pattern.MATCH => ex u)
-      | Abs (_, _, t) => ex t
-      | _ => raise MATCH);
-  in ex t2 end;
-
-fun unfold_def thy ctxt def = 
-  let 
-    val thm_lhs = get_def_thm_lhs thy def 
-    val raw_game_cterm = get_def_thm_rhs thy def |> Thm.cterm_of ctxt
-    val tables = match_subterms ctxt thm_lhs def
-    val game_cterm = Thm.instantiate_beta_cterm tables raw_game_cterm
-    val game = Thm.term_of game_cterm
-  in
-    game
-  end
-
-(* deconstructs term combination until a subterm in t2 matches t1 *)
-fun match_combs ctxt t1 t2 =
-    let
-        fun match_helper t2 =
-            (Thm.match (Thm.cterm_of ctxt t1, Thm.cterm_of ctxt t2);
-             [])
-            handle Pattern.MATCH =>
-                (case t2 of
-                    t $ u => u :: match_helper t
-                  | Abs (_, _, t) => match_helper t
-                  | _ => [])
-    in
-       match_helper t2 |> rev
-    end;
-
-fun get_combs thy ctxt def =
-  let 
-    val thm_lhs = get_def_thm_lhs thy def 
-    val tables = match_subterms ctxt thm_lhs def
-    val thm_lhs_cterm = Thm.cterm_of ctxt thm_lhs
-    val lhs = Thm.instantiate_beta_cterm tables thm_lhs_cterm
-    val combs = match_combs ctxt (Thm.term_of lhs) def
-  in
-    combs
-  end
-
-fun agm_combs (c::combs) (adv::advs) (agm::agm_advs) (extr::extrs) = 
-  if c=adv 
-  then agm::agm_combs combs advs agm_advs (extr::extrs)
-  else if c=extr
-       then extr::agm_combs combs (adv::advs) (agm::agm_advs) extrs 
-       else agm_combs combs (adv::advs) (agm::agm_advs) (extr::extrs)
-  | agm_combs (c::combs) (adv::advs) (agm::agm_advs) extrs =  
-  if c=adv 
-  then agm::agm_combs combs advs agm_advs extrs
-  else agm_combs combs (adv::advs) (agm::agm_advs) extrs
-  | agm_combs (c::combs) advs agm_advs (extr::extrs) = 
-  if c=extr 
-  then extr::agm_combs combs advs agm_advs extrs 
-  else agm_combs combs advs agm_advs (extr::extrs)
-  | agm_combs combs _ _ _ = combs
-  
-exception ADV_PARAM;
-
-(* combs with the adversary lifted type to an algebraic algorithm *)
-fun lift_to_agmT ctxt grp_desc combs advs extrs = 
-  let 
-    val nctxt = Variable.names_of ctxt
-    val grpT = Term.fastype_of grp_desc |> Term.dest_Type_args |> hd;
-    val vecT = @{typ "int list"}
-    val agm_advs = map (fn (Term.Free(name,T)) => (Term.Free(name, lift_to_algebraicT grpT vecT T)) | _ => raise ADV_PARAM) advs
-    val combs' = agm_combs combs advs agm_advs extrs
-  in 
-    combs'
-  end
-
-exception AGMTYPE1;
-exception AGMTYPE2 of typ*(string*typ);
-
-fun repair_agmT_abs nctxt (\<^Type>\<open>Product_Type.prod T1 T2\<close>) (Const ("Product_Type.prod.case_prod", T3) $ t) T2list
-  = let 
-      val (fixed_t, nctxt', agm_vars) = repair_agmT_abs nctxt T1 t (T2::T2list)
-      val retT = Term.body_type T3
-    in 
-       (\<^Const>\<open>Product_Type.prod.case_prod T1 T2 retT\<close> $ fixed_t, nctxt', agm_vars)
-    end
-  | repair_agmT_abs nctxt (\<^Type>\<open>Product_Type.prod T1 T2\<close>) (Abs(aN,aT,t)) T2list = 
-      if T1 = aT andalso T2 = @{typ "int list"} then 
-        let 
-          val (vecN,nctxt') = Name.variant (aN ^ "vec") nctxt 
-          val (fixed_t, nctxt'', agm_vars) = case T2list of (T2::T2tl) => repair_agmT_abs nctxt' T2 t T2tl
-          | [] => (t,nctxt, [])
-          val retT = Term.fastype_of t
-          val vec = Free (vecN,T2)
-          val agm_var = (Free(aN,aT), vec)
-          val abs_vec = fixed_t |> Term.incr_boundvars 1 |> Term.lambda vec
-        in
-          (\<^Const>\<open>Product_Type.prod.case_prod T1 T2 retT\<close> $ Abs(aN, aT, abs_vec), nctxt'', agm_var::agm_vars)
-        end
-      else raise AGMTYPE1
-  | repair_agmT_abs nctxt T1 (Abs(varN, varT, t)) (T2::T2list) =
-    if T1 <> varT then 
-      raise AGMTYPE2(T1, (varN,varT))
-    else 
-      let 
-        val (fixed_t, nctxt', agm_vars) = repair_agmT_abs nctxt T2 t T2list
-      in
-        (Abs(varN, varT, fixed_t), nctxt',agm_vars)
-      end
-  | repair_agmT_abs nctxt _ t  _ = (t,nctxt,[])
-  
-
-fun repair_agm_abs nctxt spmf abs = 
-  let 
-    val spmfT = Term.head_of spmf |> Term.fastype_of |> Term.body_type |> strip_spmfT
-  in
-    repair_agmT_abs nctxt spmfT abs []
-  end
-
-fun repair_agm_abss grpT nctxt t advs = 
-  case t of 
-    Const("SPMF.bind_spmf",bindT) $ spmf $ abs => 
-    let 
-      val (fixed_abs,nctxt', agm_vars) = repair_agm_abss grpT nctxt abs advs
-    in 
-      if List.exists (fn a => Term.head_of spmf = a) advs then 
-        let 
-          val (fix,nctxt'', agm_vars') = repair_agm_abs nctxt' spmf fixed_abs
-          val bindT_fix = Term.map_atyps (adjoin grpT @{typ "int list"}) bindT
-        in 
-          (Const("SPMF.bind_spmf",bindT_fix) $ spmf $ fix, nctxt'', agm_vars' @ agm_vars) 
-        end
-        else (Const("SPMF.bind_spmf",bindT) $ spmf $ fixed_abs, nctxt', agm_vars) 
-    end
-  | Abs(aT,aN,t) => 
-    let 
-      val (fixed_t, nctxt', agm_vars) = repair_agm_abss grpT nctxt t advs
-    in 
-      (Abs(aT,aN,fixed_t),nctxt', agm_vars)
-    end
-   | t1 $ t2 => 
-      let 
-        val (fixed_t1,nctxt', agm_vars) = repair_agm_abss grpT nctxt t1 advs;
-        val (fixed_t2,nctxt'', agm_vars') = repair_agm_abss grpT nctxt' t2 advs;
-      in 
-        ((fixed_t1 $ fixed_t2), nctxt'', agm_vars @ agm_vars')
-      end
-    | t => (t,nctxt,[])
-
-exception EXTR_FREE_VAR;
-
-fun lift_extr_to_agm extrs agm_vars (Abs(aN,aT,t)) = 
-  let 
-    val (pram,inst) = Term.dest_abs_global (Abs(aN,aT,t))
-    val res = lift_extr_to_agm extrs agm_vars inst
-    val rest = fst res
-    val extrs' = snd res
-    val var = Free(pram)
-  in 
-    (Term.lambda var rest, extrs')
-  end
-  | lift_extr_to_agm extrs agm_vars t = 
-  let
-    val (f,combs) = Term.strip_comb t
-    val extr = List.find (fn e => Term.head_of f = e) extrs
-  in
-    case extr of SOME extr => 
-    let 
-      val combs' = map (fn c => 
-        case List.find (fn (a,_) =>  a = c) agm_vars of SOME (a,avec) => 
-        let 
-          val aT = Term.fastype_of a
-          val avecT = Term.fastype_of avec
-        in
-          \<^Const>\<open>Product_Type.Pair aT avecT for a avec\<close> 
-        end
-        | NONE => c) combs
-      val f' = case extr of Free (fN, fT) => Free(fN, (map Term.fastype_of combs') ---> Term.body_type fT)
-        | _ => raise EXTR_FREE_VAR
-    in
-      (Term.list_comb (f', combs'), [f'])
-    end
-    | NONE => 
-    let 
-      val res = map (lift_extr_to_agm extrs agm_vars) combs
-      val combs' = map fst res
-      val extrs' = List.concat (map snd res)
-    in
-      (Term.list_comb (f,combs'), extrs')
-    end
-  end
-
-
-exception ADV_FREE_VAR;
-
-fun insert_agm_constraints nctxt grp_desc advs (Free(fN,fT)) = 
-  if List.exists (fn Free(aN,_) => aN = fN | _ => raise ADV_FREE_VAR) advs then
-     enforce_alg nctxt grp_desc (Free(fN,fT))
-  else Free(fN,fT)
-  | insert_agm_constraints nctxt grp_desc advs (Abs(aN,aT,t)) = 
-    (Abs(aN,aT,insert_agm_constraints nctxt grp_desc advs t))
-  | insert_agm_constraints nctxt grp_desc advs (t1 $ t2) = 
-   insert_agm_constraints nctxt grp_desc advs t1 $ (insert_agm_constraints nctxt grp_desc advs t2)
-  | insert_agm_constraints _ _ _ t = t
-
-
-fun lift_to_agm thy ctxt grp_desc def advs extrs = 
-  let 
-    val nctxt = Variable.names_of ctxt
-    val game = unfold_def thy ctxt def
-    val combs = get_combs thy ctxt def
-    val combs' = lift_to_agmT ctxt grp_desc combs advs extrs
-    val grpT = Term.fastype_of grp_desc |> Term.dest_Type_args |> hd;
-    val vecT = @{typ "int list"}
-    val agm_advs = map (fn (Term.Free(name,T)) => (Term.Free(name, lift_to_algebraicT grpT vecT T)) | _ => raise ADV_PARAM) advs
-    val game' = Term.betapplys (game,combs')
-    val (game'',_,agm_vars) = repair_agm_abss grpT nctxt game' agm_advs
-    val (game''', extrs') = lift_extr_to_agm extrs agm_vars game''
-    val combs'' = map (fn Free(combN,combT) => 
-      (case List.find (fn Free(eN,eT) => eN = combN | _ => raise ADV_FREE_VAR) extrs' 
-        of SOME e => e 
-        | NONE => Free(combN,combT)) 
-      | _ => raise ADV_FREE_VAR) combs'
-    val game'''' = insert_agm_constraints nctxt grp_desc advs game'''
-    val agm_game = fold (fn comb => fn game => Term.lambda comb game) (rev combs'') game''''
-    val agm_cterm = Thm.cterm_of ctxt agm_game
-  in
-    agm_game
-  end
-
-end;
+agm_interpretation automates the instance resolution: given a group and a function type, it 
+automatically lifts the function type via lift_to_algebraicT and interprets AlgebraicAlgorithm
+with a composed Select record, mirroring the functions (decurried) input, and Constrain record, 
+mirroring the functions output.
 \<close>
 
 text \<open>This takes any algorithm/function type and lifts it to the algebraic algorithm equivalent type.
 For examples take a look at the end of this file.\<close>
 ML \<open>
-  Outer_Syntax.local_theory \<^command_keyword>\<open>lift_to_algebraicT\<close> "lift to algebraic type"
-    (Parse.typ -- (Parse.term -- (\<^keyword>\<open>=>\<close> |--Parse.binding)) >> 
-      (fn (alg,(grp,b)) => fn lthy => Local_Theory.raw_theory (fn thy =>
-      let
-        val algT = Syntax.read_typ lthy alg;
-        val grp_desc = Syntax.read_term lthy grp;
-        val grpT = Term.fastype_of grp_desc |> Term.dest_Type_args |> hd;
-        val agmT = Algebraic_Algorithm.lift_to_algebraicT grpT @{typ "int list"} algT;
-        val tps = Algebraic_Algorithm.extract_type_params agmT;
-        val thy' = Sign.add_type_abbrev lthy (b, tps, agmT) thy
-      in thy' end) lthy));
+  local 
+    (*apply function f to the codaomain of a function*)
+    fun rcodomain_transf f (Type ("fun", [T, U])) = (Type ("fun", [T, rcodomain_transf f U]))
+      | rcodomain_transf f T = f T;
+    
+    (*adjoin vec to t as a product type if the Type = t*)
+    fun adjoin t vec = fn T => if T = t then Type ("Product_Type.prod", [T, vec]) else T
+    
+    (*decurry a function*)
+    fun decurry (Type ("fun", [T1, Type ("fun", [T2, T3])])) = 
+        decurry (Type ("fun", [Type ("Product_Type.prod", [T1, T2]), T3]))
+      | decurry T = T
+    
+    fun extract_type_params t = Term.add_tfree_namesT t []
+    
+    fun lift_to_algebraicT grpT vec = (rcodomain_transf (Term.map_atyps (adjoin grpT vec))) o decurry
+
+  in 
+  val _ = 
+    Outer_Syntax.local_theory \<^command_keyword>\<open>lift_to_algebraicT\<close> "lift to algebraic type"
+      (Parse.typ -- (Parse.term -- (\<^keyword>\<open>=>\<close> |--Parse.binding)) >> 
+        (fn (alg,(grp,b)) => fn lthy => Local_Theory.raw_theory (fn thy =>
+        let
+          val algT = Syntax.read_typ lthy alg;
+          val grp_desc = Syntax.read_term lthy grp;
+          val grpT = Term.fastype_of grp_desc |> Term.dest_Type_args |> hd;
+          val agmT = lift_to_algebraicT grpT @{typ "int list"} algT;
+          val tps = extract_type_params agmT;
+          val thy' = Sign.add_type_abbrev lthy (b, tps, agmT) thy
+        in thy' end) lthy));
+  end;
 \<close>
 
-text \<open>This takes any algorithm/function and enforces the rules of an algebraic algorithm on all 
-suitable output pairs (g,gvec).
-For examples take a look at the end of this file.\<close>
 ML \<open>
-  Outer_Syntax.local_theory \<^command_keyword>\<open>lift_to_algebraic\<close> "lift to algebraic type"
-    (Parse.term -- (Parse.term -- (\<^keyword>\<open>=>\<close> |--Parse.binding)) >> 
-      (fn (a,(grp,b)) => fn lthy => 
+  local
+    fun rcodomain_transf f (Type ("fun", [T, U])) = (Type ("fun", [T, rcodomain_transf f U]))
+      | rcodomain_transf f T = f T;
+
+    fun adjoin t vec = fn T => if T = t then Type ("Product_Type.prod", [T, vec]) else T;
+
+    fun decurry (Type ("fun", [T1, Type ("fun", [T2, T3])])) =
+        decurry (Type ("fun", [Type ("Product_Type.prod", [T1, T2]), T3]))
+      | decurry T = T;
+
+    fun lift_to_algebraicT grpT vec =
+      (rcodomain_transf (Term.map_atyps (adjoin grpT vec))) o decurry;
+
+    fun const_exists ctxt name =
       let
-        val nctxt = Variable.names_of lthy
-        val alg = Syntax.read_term lthy a;
-        val grp_desc = Syntax.read_term lthy grp;
-        val agm_term = Algebraic_Algorithm.enforce_alg nctxt grp_desc alg;
-        val (def, thy') = Local_Theory.define ((b, NoSyn), ((Thm.def_binding b, []), agm_term)) lthy;
-      in thy' end));
+        val thy = Proof_Context.theory_of ctxt;
+      in
+        can (fn n => Sign.const_type thy (Proof_Context.intern_const ctxt n)) name
+      end;
+
+    fun mk_select ctxt grpT grp_s T =
+      if T = grpT then "cyclic_group.groupS"
+      else
+        (case T of
+          Type ("Product_Type.prod", [A, B]) =>
+            "prodS (" ^ mk_select ctxt grpT grp_s A ^ ") (" ^ mk_select ctxt grpT grp_s B ^ ")"
+        | Type (tycon, args) =>
+            let
+              val ctor = Long_Name.base_name tycon ^ "S";
+            in
+              if const_exists ctxt ctor then
+                fold (fn arg => fn acc => acc ^ " (" ^ mk_select ctxt grpT grp_s arg ^ ")") args ctor
+              else "noSelect"
+            end
+        | _ => "noSelect");
+
+    fun mk_constrain ctxt grpT vecT grp_s T =
+      (case T of
+        Type ("Product_Type.prod", [A, B]) =>
+          if A = grpT andalso B = vecT then "(cyclic_group.groupC " ^ grp_s ^ ")"
+          else "prodC (" ^ mk_constrain ctxt grpT vecT grp_s A ^ ") (" ^ mk_constrain ctxt grpT vecT grp_s B ^ ")"
+      | Type (tycon, args) =>
+          let
+            val ctor = Long_Name.base_name tycon ^ "C";
+          in
+            if const_exists ctxt ctor then
+              fold (fn arg => fn acc => acc ^ " (" ^ mk_constrain ctxt grpT vecT grp_s arg ^ ")") args ctor
+            else "noConstrain"
+          end
+      | _ => "noConstrain");
+
+    fun mk_unfold_locales_method_range () : Method.text_range =
+      let
+        val src = Token.make_src ("unfold_locales", Position.none) [];
+      in
+        (Method.Source src, Position.no_range)
+      end;
+
+    fun strip_markup s =
+      let
+        val X = #"\005";
+        fun go [] _ acc = String.implode (rev acc)
+          | go (c :: cs) in_tag acc =
+              if in_tag then
+                if c = X then go cs false acc else go cs true acc
+              else if c = X then go cs true acc
+              else go cs false (c :: acc);
+      in
+        go (String.explode s) false []
+      end;
+
+    fun safe_term_source ctxt t =
+      strip_markup (Syntax.string_of_term ctxt t);
+
+    fun mk_alg_expr (b: binding) (g: string) (sel: string) (con: string) : Expression.expression =
+      let
+        val prefix = (Binding.name_of b, true);
+        val inst = Expression.Positional [SOME g, SOME sel, SOME con];
+        val expr = [(("Algebraic_Algorithm", Position.none), (prefix, (inst, [])))];
+      in
+        (expr, [])
+      end;
+  in
+    val _ =
+      Outer_Syntax.command \<^command_keyword>\<open>agm_interpretation\<close>
+        "interpret Algebraic_Algorithm and discharge obligations via unfold_locales"
+        (Parse.binding --| \<^keyword>\<open>:\<close> -- Parse.term -- Parse.typ >>
+          (fn ((b, g), alg_ty) =>
+            let
+              val m = mk_unfold_locales_method_range ();
+              fun interp lthy =
+                let
+                  val algT = Syntax.read_typ lthy alg_ty;
+                  val grp_desc = Syntax.read_term lthy g;
+                  val grp_s =
+                    (case try (fn () => safe_term_source lthy grp_desc) () of
+                      SOME s => s
+                    | NONE => strip_markup g);
+                  val grpT = Term.fastype_of grp_desc |> Term.dest_Type_args |> hd;
+                  val vecT = @{typ "int list"};
+                  val agmT = lift_to_algebraicT grpT vecT algT;
+                  val (inps, resT) = Term.strip_type agmT;
+                  val inpT =
+                    (case inps of
+                      [] => error "agm_interpretation: expected function type"
+                    | T :: Ts =>
+                        fold (fn U => fn acc => Type ("Product_Type.prod", [acc, U])) Ts T);
+                  val outT =
+                    let
+                      val thy = Proof_Context.theory_of lthy;
+                      val out_ix = ("out", 0);
+                      val out_tv = (out_ix, @{sort type});
+                      val spmf_pat =
+                        Term.map_atyps (K (TVar out_tv)) @{typ "'a spmf"};
+                    in
+                      (case try (fn () => Sign.typ_match thy (spmf_pat, resT) Vartab.empty) () of
+                        SOME tyenv =>
+                          (case Vartab.lookup tyenv out_ix of
+                            SOME (_, T) => T
+                          | NONE =>
+                              error
+                                ("agm_interpretation: internal error (failed to recover spmf type argument)"))
+                      | NONE =>
+                          error
+                            ("agm_interpretation: expected lifted type with codomain _ spmf, got: " ^
+                             Syntax.string_of_typ lthy resT ^ " in " ^ Syntax.string_of_typ lthy agmT))
+                    end;
+                  val sel_s = mk_select lthy grpT grp_s inpT;
+                  val con_s = mk_constrain lthy grpT vecT grp_s outT;
+                  val expr = mk_alg_expr b grp_s sel_s con_s;
+                in
+                  Interpretation.isar_interpretation_cmd expr lthy
+                end;
+            in
+              Toplevel.local_theory_to_proof NONE NONE interp
+              #> Toplevel.proofs (Proof.apply_end m)
+              #> Toplevel.proof Proof.local_done_proof
+            end))
+  end;
 \<close>
 
-text \<open>This takes any function/algorithm type T and computes a function that enforces the algebraic 
-algorithm rules on concrete algorithms of the algebraic algorithm equivalent type of T. To be used 
-to turn adversaries from the standard model into the algebraic group model.
-For examples take a look at the end of this file.\<close>
-ML \<open>
-  Outer_Syntax.local_theory \<^command_keyword>\<open>AGMLifting\<close> "lift to algebraic type"
-    (Parse.typ -- (Parse.term -- (\<^keyword>\<open>=>\<close> |--Parse.binding)) >> 
-      (fn (adv,(grp,b)) => fn lthy =>
-      let
-        val nctxt = Variable.names_of lthy
-        val advT = Syntax.read_typ lthy adv;
-        val grp_desc = Syntax.read_term lthy grp;
-        val grpT = Term.fastype_of grp_desc |> Term.dest_Type_args |> hd;
-        val agm_advT = Algebraic_Algorithm.lift_to_algebraicT grpT @{typ "int list"} advT;
-        val agm_term = Algebraic_Algorithm.build_alg_fun nctxt grp_desc agm_advT;
-        val (def, thy') = Local_Theory.define ((b, NoSyn), ((Thm.def_binding b, []), agm_term)) lthy;
-      in thy' end));
-\<close>
+subsection \<open>Examples for the ML functions\<close>
 
-text \<open>This takes a game in the standard model and lifts it into the AGM.
-Syntax: Group game | adversaries | extra(ctors) = *new_game_name*
-The game should be supplied with free variable parameters. A subset of these parameters will be the 
-adversaries, which may be explicitly lifted into the AGM by listing them in the "adversaries" 
-section, separated by commas - the same applies to the extra(ctors) (typically extractors), which 
-are algorithms that should also receive the AGM vector for values from a adversary. 
-For an Example take a look at KZG_knowledge_soundness.thy\<close>
-ML \<open>
-  Outer_Syntax.local_theory \<^command_keyword>\<open>lift_to_AGM\<close> "lift game to Algeraic Group Model"
-    (Parse.term -- (Parse.term -- (\<^keyword>\<open>|\<close> |-- ((Parse.enum "," Parse.term ) -- 
-      (\<^keyword>\<open>|\<close> |-- ((Parse.enum "," Parse.term ) -- (\<^keyword>\<open>=\<close> |-- Parse.binding)))))) >> 
-      (fn (grp,(game_name,(advl, (extrl,b)))) => fn lthy => 
-      let
-        val thy = Proof_Context.theory_of lthy;
-        val game_ref = Syntax.read_term lthy game_name;
-        val advs = Syntax.read_terms lthy advl;
-        val extrs = Syntax.read_terms lthy extrl;
-        val grp_desc = Syntax.read_term lthy grp;
-        val agm_term = Algebraic_Algorithm.lift_to_agm thy lthy grp_desc game_ref advs extrs;
-        val (def, lthy') = Local_Theory.define ((b, NoSyn), ((Thm.def_binding b, []), agm_term)) lthy;
-      in lthy' end));
-\<close>
-
-subsection \<open>Examples\<close>
-
-text\<open>Example to enforce the algebraic rules on an arbitrary adversary.\<close>
-
+text \<open>We define a standard model adversary with group G of type 'a\<close>
 type_synonym ('a')adv = "'a' list \<Rightarrow> 'a' \<Rightarrow> nat \<Rightarrow> ('a' * int * nat) spmf"
 
-declare [[show_types]]
-AGMLifting  "('a) adv" "G" => agm_adv
-thm agm_adv_def
+text \<open>We lift the type into the AGM (its algebraic algorithm pendant):\<close>
+lift_to_algebraicT "('a) adv"  "G" => algebraic_adv
 
-lift_to_algebraicT "('a)adv" G => agm_advT
 
-ML \<open>
-val agm_adv_typ = @{typ "('a)agm_advT"}
-\<close>
+text \<open>We interpret restrict for the created algebraic_adv\<close>
+interpretation manualAGM: Algebraic_Algorithm G "prodS (prodS (listS groupS) groupS) noSelect" 
+  "prodC groupC (prodC noConstrain noConstrain)"
+  by (unfold_locales)
 
-lemma "agm_adv \<equiv> \<lambda>(A::('a)agm_advT) a b c. do { 
-      ((g,gvec),e,d) \<leftarrow> A a b c;
-      _::unit \<leftarrow> assert_spmf((length (a @ [b]) = length gvec 
-        \<and> g = fold (\<lambda> i acc. acc \<otimes> (a @ [b])!i [^] (gvec!i)) [0..<length (a @ [b])] \<one>));
-      return_spmf ((g,gvec),e,d) 
-    }"
-  unfolding agm_adv_def by fastforce
+text \<open>We skip the last step and automatically interpret the right version restrict version 
+for adv.\<close>
+agm_interpretation autoAGM : G "('a)adv" ..
 
-text \<open>Example to enforce algebraic rules on the outputs of a specific adversary of correct type\<close>
-
-definition \<A>::"('a) agm_advT"
-  where "\<A> a b c = return_spmf((\<one>,[0,0]),-1,1)"
-
-lift_to_algebraic \<A> G => \<A>_algebraic
-thm \<A>_algebraic_def
-
-lemma 
-  "\<A>_algebraic \<equiv> \<lambda>a b c. do { 
-      ((g,gvec),e,d) \<leftarrow> \<A> a b c;
-      _::unit \<leftarrow> assert_spmf((length (a @ [b]) = length gvec 
-        \<and> g = fold (\<lambda> i acc. acc \<otimes> (a @ [b])!i [^] (gvec!i)) [0..<length (a @ [b])] \<one>));
-      return_spmf ((g,gvec),e,d) 
-    }"
-  unfolding \<A>_algebraic_def by fastforce
-
-text \<open>For an example to lift a game into the AGM take a look at KZG_knowledge_soundness.thy\<close>
+lemma "manualAGM.restrict = autoAGM.restrict"
+  unfolding manualAGM.restrict_def autoAGM.restrict_def
+  by simp
+  
 
 end
 
